Differentiate parity examples (#312)
* rename Parity to ParitySingle and differentiate module description from ParityComposition

* differentiate ParityComposition constants from ParitySingle using mul prefix

* move app_valid_tran tactic to VLSM module

* rename simple example to Parity and composition example to PrimesComposition

* avoid using Component as part of names in VLSM example definitions

* change ParityValid to Parity_valid

theories/VLSM/Core/Examples/PrimesComposition.v
@@ -6,60 +6,48 @@ From VLSM.Lib Require Import Preamble StdppExtras FinSuppFn NatExtras ListExtras
 From VLSM.Core Require Import VLSM PreloadedVLSM ConstrainedVLSM Composition.
 From VLSM.Core Require Import VLSMProjections ProjectionTraces.
 
-(** * Parity VLSM
+(** * Primes Composition of VLSMs
 
-  This module demonstrates some basic notions of the VLSM framework.
-  The idea of the parity VLSM is to store an integer and continually decrement it,
-  while a constraint is checked at each step. The definitions and lemmas tap into
-  concepts such as valid and constrained traces, transitions, states, and messages.
+  This module demonstrates advanced concepts of the VLSM framework. We define
+  a radix VLSM parameterized on a multiplier and a composition
+  of such VLSMs. We then construct the composition consisting of a component
+  for each prime number, characterize the valid messages, and show that any
+  component in the composition is a validator.
 *)
 
 #[local] Open Scope Z_scope.
 
-(** ** General automation *)
+Section sec_radix_vlsm.
 
-(** Custom tactic used to simplify proofs of valid VLSM transitions. *)
-
-Ltac app_valid_tran :=
-  repeat split; cbn;
-  match goal with
-  | |- option_valid_message_prop _ _ => by apply initial_message_is_valid
-  | |- option_valid_message_prop _ _ => eapply emitted_messages_are_valid
-  | |- valid_state_prop _ _ => by apply initial_state_is_valid
-  | |- valid_state_prop _ _ => eapply input_valid_transition_destination
-  end.
-
-Section sec_parity_vlsm.
-
+(**
+  We parameterize a radix VLSM on an integer multiplier
+  greater than one.
+*)
 Context
  (multiplier : Z)
  (multiplier_gt_1 : multiplier > 1)
- (index : Type)
- `{Inhabited index}
  .
 
-(** ** Definition of Parity VLSM
+(** ** Definition of the Radix VLSM
 
-  The Parity VLSM will only have one label, indicating a decrement.
+  The Radix VLSM will only have one label, indicating a decrement.
   For this reason, the [unit] type can be used.
 *)
 
-Definition ParityLabel : Type := unit.
+Definition RadixLabel : Type := unit.
 
-(** The state will hold an integer. *)
+(** The state holds an integer. *)
 
-Definition ParityState : Type := Z.
+Definition RadixState : Type := Z.
 
 (** Messages are integers. *)
 
-Definition ParityMessage : Type := Z.
+Definition RadixMessage : Type := Z.
 
-(** A VLSM Type is defined using ParityState and ParityLabel. *)
-
-Definition ParityType : VLSMType ParityMessage :=
+Definition RadixType : VLSMType RadixMessage :=
 {|
-  state := ParityState;
-  label := ParityLabel;
+  state := RadixState;
+  label := RadixLabel;
 |}.
 
 (**
@@ -67,18 +55,18 @@ Definition ParityType : VLSMType ParityMessage :=
   and guard predicate are as follows:
 *)
 
-Definition ParityComponent_initial_state_prop (st : ParityState) : Prop := st >= 1.
+Definition Radix_initial_state_prop (st : RadixState) : Prop := st >= 1.
 
-Definition ParityComponent_transition
-  (l : ParityLabel) (st : ParityState) (om : option ParityMessage)
-  : ParityState * option ParityMessage :=
+Definition Radix_transition
+  (l : RadixLabel) (st : RadixState) (om : option RadixMessage)
+  : RadixState * option RadixMessage :=
   match om with
   | Some j  => (st - j, Some (multiplier * j))
   | None    => (st, None)
   end.
 
-Definition ParityComponent_valid
-  (l : ParityLabel) (st : ParityState) (om : option ParityMessage) : Prop :=
+Definition Radix_valid
+  (l : RadixLabel) (st : RadixState) (om : option RadixMessage) : Prop :=
   match om with
   | Some msg => msg <= st /\ 2 <= msg
   | None     => False
@@ -89,53 +77,53 @@ Definition ParityComponent_valid
   is inhabited as the set of initial states is non-empty.
 *)
 
-Definition ParityComponent_initial_state_type : Type :=
-  {st : ParityState | ParityComponent_initial_state_prop st}.
+Definition Radix_initial_state_type : Type :=
+  {st : RadixState | Radix_initial_state_prop st}.
 
-Program Definition ParityComponent_initial_state :
-  ParityComponent_initial_state_type := exist _ 1 _.
+Program Definition Radix_initial_state :
+  Radix_initial_state_type := exist _ 1 _.
 Next Obligation.
 Proof. done. Defined.
 
-#[export] Instance ParityComponent_Inhabited_initial_state_type :
-  Inhabited (ParityComponent_initial_state_type) :=
-    populate (ParityComponent_initial_state).
+#[export] Instance Radix_Inhabited_initial_state_type :
+  Inhabited (Radix_initial_state_type) :=
+    populate (Radix_initial_state).
 
 (**
   An intermediate representation for the VLSM is required.
   It uses the previously defined specifications.
 *)
 
-Definition ParityMachine : VLSMMachine ParityType :=
+Definition RadixMachine : VLSMMachine RadixType :=
 {|
-  initial_state_prop := ParityComponent_initial_state_prop;
-  initial_message_prop := fun (ms : ParityMessage) => ms = multiplier;
-  s0 := ParityComponent_Inhabited_initial_state_type;
-  transition := fun l '(st, om) => ParityComponent_transition l st om;
-  valid := fun l '(st, om) => ParityComponent_valid l st om;
+  initial_state_prop := Radix_initial_state_prop;
+  initial_message_prop := fun (ms : RadixMessage) => ms = multiplier;
+  s0 := Radix_Inhabited_initial_state_type;
+  transition := fun l '(st, om) => Radix_transition l st om;
+  valid := fun l '(st, om) => Radix_valid l st om;
 |}.
 
-(** The definition of the Parity VLSM. *)
+(** The definition of the Radix VLSM. *)
 
-Definition ParityVLSM : VLSM ParityMessage :=
+Definition RadixVLSM : VLSM RadixMessage :=
 {|
-  vtype := ParityType;
-  vmachine := ParityMachine;
+  vtype := RadixType;
+  vmachine := RadixMachine;
 |}.
 
 (**
-  To improve readability, we explicitly define [parity_label] as the value of
+  To improve readability, we explicitly define [radix_label] as the value of
   the unit type.
 *)
 
-Definition parity_label : label ParityType := ().
+Definition radix_label : label RadixType := ().
 
-(** ** Parity VLSM Examples *)
+(** ** Radix VLSM Examples *)
 
 (** *** Example of an arbitrary transition *)
 
-Lemma parity_example_transition_1 `(X : VLSM ParityMessage) :
-  transition ParityVLSM parity_label (4, Some 10) = (-6, Some (multiplier * 10)).
+Lemma radix_example_transition_1 `(X : VLSM RadixMessage) :
+  transition RadixVLSM radix_label (4, Some 10) = (-6, Some (multiplier * 10)).
 Proof. done. Qed.
 
 (** *** Example of a valid trace *)
@@ -149,203 +137,207 @@ Proof. done. Qed.
   difference to the trace.
 *)
 
-Definition parity_trace1_init : list (transition_item ParityVLSM) :=
-  [ Build_transition_item parity_label (Some (multiplier ^ 2))
+Definition radix_trace1_init : list (transition_item RadixVLSM) :=
+  [ Build_transition_item radix_label (Some (multiplier ^ 2))
      (multiplier ^ 3 - multiplier ^ 2) (Some (multiplier ^ 3))
-  ; Build_transition_item parity_label (Some multiplier)
+  ; Build_transition_item radix_label (Some multiplier)
      (multiplier ^ 3 - multiplier ^ 2 - multiplier) (Some (multiplier ^ 2)) ].
 
-Definition parity_trace1_last_item : transition_item ParityVLSM :=
-  Build_transition_item parity_label (Some multiplier)
+Definition radix_trace1_last_item : transition_item RadixVLSM :=
+  Build_transition_item radix_label (Some multiplier)
     (multiplier ^ 3 - multiplier ^ 2 - multiplier - multiplier) (Some (multiplier ^ 2)).
 
-Definition parity_trace1 : list (transition_item ParityVLSM) :=
-  parity_trace1_init ++ [parity_trace1_last_item].
+Definition radix_trace1 : list (transition_item RadixVLSM) :=
+  radix_trace1_init ++ [radix_trace1_last_item].
 
-Definition parity_trace1_first_state : ParityState := multiplier ^ 3.
+Definition radix_trace1_first_state : RadixState := multiplier ^ 3.
 
-Definition parity_trace1_last_state : ParityState :=
-  destination parity_trace1_last_item.
+Definition radix_trace1_last_state : RadixState :=
+  destination radix_trace1_last_item.
 
 (** The trace we defined is valid: *)
 
-Example parity_valid_message_prop_mult :
-  valid_message_prop ParityVLSM multiplier.
+Example radix_valid_message_prop_mult :
+  valid_message_prop RadixVLSM multiplier.
 Proof. by apply initial_message_is_valid. Qed.
 
-Example parity_can_emit_square_mult :
-  can_emit ParityVLSM (multiplier ^ 2).
+Example radix_can_emit_square_mult :
+  can_emit RadixVLSM (multiplier ^ 2).
 Proof.
-  exists (multiplier, Some multiplier), parity_label, 0.
+  exists (multiplier, Some multiplier), radix_label, 0.
   repeat split; [| | by lia.. | by cbn; do 2 f_equal; lia].
-  - by apply initial_state_is_valid; cbn; unfold ParityComponent_initial_state_prop; lia.
+  - by apply initial_state_is_valid; cbn; unfold Radix_initial_state_prop; lia.
   - by app_valid_tran.
 Qed.
 
-Example parity_valid_message_prop_square_mult :
-  valid_message_prop ParityVLSM (multiplier ^ 2).
+Example radix_valid_message_prop_square_mult :
+  valid_message_prop RadixVLSM (multiplier ^ 2).
 Proof.
-  by eapply emitted_messages_are_valid, parity_can_emit_square_mult.
+  by eapply emitted_messages_are_valid, radix_can_emit_square_mult.
 Qed.
 
-Proposition parity_valid_transition_1 :
-  input_valid_transition ParityVLSM parity_label
-   (parity_trace1_first_state, Some (multiplier ^ 2))
+Proposition radix_valid_transition_1 :
+  input_valid_transition RadixVLSM radix_label
+   (radix_trace1_first_state, Some (multiplier ^ 2))
    (multiplier ^ 3 - multiplier ^ 2, Some (multiplier ^ 3)).
 Proof.
   repeat split; [| | | by lia].
   - by apply initial_state_is_valid; cbn;
-      unfold ParityComponent_initial_state_prop, parity_trace1_first_state; lia.
-  - by app_valid_tran; eapply parity_can_emit_square_mult.
-  - by unfold parity_trace1_first_state; nia.
+      unfold Radix_initial_state_prop, radix_trace1_first_state; lia.
+  - by app_valid_tran; eapply radix_can_emit_square_mult.
+  - by unfold radix_trace1_first_state; nia.
 Qed.
 
-Proposition parity_valid_transition_2 :
+Proposition radix_valid_transition_2 :
   multiplier >= 2 ->
-  input_valid_transition ParityVLSM parity_label
+  input_valid_transition RadixVLSM radix_label
    (multiplier ^ 3 - multiplier ^ 2, Some multiplier)
    (multiplier ^ 3 - multiplier ^ 2 - multiplier, Some (multiplier ^ 2)).
 Proof.
   repeat split; [| | | by lia |].
-  - by app_valid_tran; eapply parity_valid_transition_1; lia.
-  - by app_valid_tran; apply parity_can_emit_square_mult.
+  - by app_valid_tran; eapply radix_valid_transition_1; lia.
+  - by app_valid_tran; apply radix_can_emit_square_mult.
   - by nia.
   - by cbn; do 2 f_equal; lia.
 Qed.
 
-Proposition parity_valid_transition_3 :
+Proposition radix_valid_transition_3 :
   multiplier >= 2 ->
-  input_valid_transition ParityVLSM parity_label
+  input_valid_transition RadixVLSM radix_label
    (multiplier ^ 3 - multiplier ^ 2 - multiplier, Some multiplier)
    (multiplier ^ 3 - multiplier ^ 2 - multiplier - multiplier, Some (multiplier ^ 2)).
 Proof.
   repeat split; [| | | by lia |].
-  - by app_valid_tran; apply parity_valid_transition_2.
-  - by app_valid_tran; apply parity_can_emit_square_mult.
+  - by app_valid_tran; apply radix_valid_transition_2.
+  - by app_valid_tran; apply radix_can_emit_square_mult.
   - by nia.
   - by cbn; do 2 f_equal; lia.
 Qed.
 
-Example parity_valid_trace1 :
+Example radix_valid_trace1 :
   multiplier >= 2 ->
-  finite_valid_trace_init_to ParityVLSM
-    parity_trace1_first_state parity_trace1_last_state parity_trace1.
+  finite_valid_trace_init_to RadixVLSM
+    radix_trace1_first_state radix_trace1_last_state radix_trace1.
 Proof.
-  constructor; unfold parity_trace1_first_state;
-    [| by cbn; unfold ParityComponent_initial_state_prop; lia].
+  constructor; unfold radix_trace1_first_state;
+    [| by cbn; unfold Radix_initial_state_prop; lia].
   repeat apply finite_valid_trace_from_to_extend.
   - by eapply finite_valid_trace_from_to_empty, input_valid_transition_destination,
-      parity_valid_transition_3.
-  - by apply parity_valid_transition_3.
-  - by apply parity_valid_transition_2.
-  - by apply parity_valid_transition_1; lia.
+      radix_valid_transition_3.
+  - by apply radix_valid_transition_3.
+  - by apply radix_valid_transition_2.
+  - by apply radix_valid_transition_1; lia.
 Qed.
 
-Example parity_valid_trace1_alt :
+Example radix_valid_trace1_alt :
   multiplier >= 2 ->
-  finite_valid_trace_init_to_alt ParityVLSM
-    parity_trace1_first_state parity_trace1_last_state parity_trace1.
+  finite_valid_trace_init_to_alt RadixVLSM
+    radix_trace1_first_state radix_trace1_last_state radix_trace1.
 Proof.
-  constructor; [| by unfold parity_trace1_first_state; cbn; red; lia].
+  constructor; [| by unfold radix_trace1_first_state; cbn; red; lia].
   repeat apply mvt_extend; [.. | by apply mvt_empty].
-  - by eapply parity_valid_message_prop_square_mult; lia.
-  - by eapply parity_valid_transition_1; lia.
+  - by eapply radix_valid_message_prop_square_mult; lia.
+  - by eapply radix_valid_transition_1; lia.
   - cbn; split; [| by lia].
-    by unfold parity_trace1_first_state; nia.
-  - by apply parity_valid_message_prop_mult.
-  - by apply parity_valid_transition_2.
+    by unfold radix_trace1_first_state; nia.
+  - by apply radix_valid_message_prop_mult.
+  - by apply radix_valid_transition_2.
   - by cbn; split; [nia | lia].
-  - by apply parity_valid_message_prop_mult.
-  - by apply parity_valid_transition_3.
+  - by apply radix_valid_message_prop_mult.
+  - by apply radix_valid_transition_3.
   - by cbn; split; [nia | lia].
 Qed.
 
 (** *** Example of a constrained trace *)
 
 (** The previously defined trace is obviously constrained, since it's valid. *)
-Lemma parity_constrained_trace1 :
+Lemma radix_constrained_trace1 :
   multiplier >= 2 ->
-  finite_constrained_trace_init_to_direct ParityVLSM
-    parity_trace1_first_state parity_trace1_last_state parity_trace1.
+  finite_constrained_trace_init_to_direct RadixVLSM
+    radix_trace1_first_state radix_trace1_last_state radix_trace1.
 Proof.
-  constructor; [| by unfold parity_trace1_first_state; cbn; red; lia].
+  constructor; [| by unfold radix_trace1_first_state; cbn; red; lia].
   repeat apply ct_extend; [.. | by apply ct_empty].
-  - by eapply parity_valid_transition_1; lia.
+  - by eapply radix_valid_transition_1; lia.
   - cbn; split; [| by lia].
-    by unfold parity_trace1_first_state; nia.
-  - by apply parity_valid_transition_2.
+    by unfold radix_trace1_first_state; nia.
+  - by apply radix_valid_transition_2.
   - by cbn; split; [nia | lia].
-  - by apply parity_valid_transition_3.
+  - by apply radix_valid_transition_3.
   - by cbn; split; [nia | lia].
 Qed.
 
-Definition parity_trace2_init : list (transition_item ParityVLSM) :=
-  [ Build_transition_item parity_label (Some multiplier) (2 * multiplier + 1) (Some (multiplier ^ 2))
-  ; Build_transition_item parity_label (Some multiplier) (multiplier + 1) (Some (multiplier ^ 2)) ].
+Definition radix_trace2_init : list (transition_item RadixVLSM) :=
+  [ Build_transition_item radix_label (Some multiplier)
+      (2 * multiplier + 1) (Some (multiplier ^ 2))
+  ; Build_transition_item radix_label (Some multiplier)
+      (multiplier + 1) (Some (multiplier ^ 2)) ].
 
-Definition parity_trace2_last_item : transition_item ParityVLSM :=
-  Build_transition_item parity_label (Some (multiplier + 1)) 0 (Some (multiplier ^ 2 + multiplier) ).
+Definition radix_trace2_last_item : transition_item RadixVLSM :=
+  Build_transition_item radix_label (Some (multiplier + 1))
+    0 (Some (multiplier ^ 2 + multiplier) ).
 
-Definition parity_trace2 : list (transition_item ParityVLSM) :=
-  parity_trace2_init ++ [parity_trace2_last_item].
+Definition radix_trace2 : list (transition_item RadixVLSM) :=
+  radix_trace2_init ++ [radix_trace2_last_item].
 
-Definition parity_trace2_init_first_state : ParityState := 3 * multiplier + 1.
+Definition radix_trace2_init_first_state : RadixState := 3 * multiplier + 1.
 
-Definition parity_trace2_init_last_state : ParityState := multiplier + 1.
+Definition radix_trace2_init_last_state : RadixState := multiplier + 1.
 
-Definition parity_trace2_last_state : ParityState :=
-  destination parity_trace2_last_item.
+Definition radix_trace2_last_state : RadixState :=
+  destination radix_trace2_last_item.
 
 (** The given trace is valid without the last transition. *)
 
-Proposition parity_valid_transition_1' :
-  input_valid_transition ParityVLSM parity_label
-    (parity_trace2_init_first_state, Some multiplier) (2 * multiplier + 1, Some (multiplier ^ 2)).
+Proposition radix_valid_transition_1' :
+  input_valid_transition RadixVLSM radix_label
+    (radix_trace2_init_first_state, Some multiplier)
+    (2 * multiplier + 1, Some (multiplier ^ 2)).
 Proof.
   repeat split; [| | | by lia |].
   - apply initial_state_is_valid.
-    by unfold parity_trace2_init_first_state; cbn; red; lia.
-  - by app_valid_tran; apply parity_can_emit_square_mult.
-  - by unfold parity_trace2_init_first_state; lia.
-  - by cbn; do 2 f_equal; unfold parity_trace2_init_first_state; lia.
+    by unfold radix_trace2_init_first_state; cbn; red; lia.
+  - by app_valid_tran; apply radix_can_emit_square_mult.
+  - by unfold radix_trace2_init_first_state; lia.
+  - by cbn; do 2 f_equal; unfold radix_trace2_init_first_state; lia.
 Qed.
 
-Proposition parity_valid_transition_2' :
-  input_valid_transition ParityVLSM parity_label
+Proposition radix_valid_transition_2' :
+  input_valid_transition RadixVLSM radix_label
     (2 * multiplier + 1, Some multiplier) (multiplier + 1, Some (multiplier ^ 2)).
 Proof.
   repeat split; [| | | by lia |].
   - apply initial_state_is_valid.
-    by unfold parity_trace2_init_first_state; cbn; red; lia.
-  - by app_valid_tran; apply parity_can_emit_square_mult.
-  - by unfold parity_trace2_init_first_state; lia.
-  - by cbn; do 2 f_equal; unfold parity_trace2_init_first_state; lia.
+    by unfold radix_trace2_init_first_state; cbn; red; lia.
+  - by app_valid_tran; apply radix_can_emit_square_mult.
+  - by unfold radix_trace2_init_first_state; lia.
+  - by cbn; do 2 f_equal; unfold radix_trace2_init_first_state; lia.
 Qed.
 
-Example parity_valid_trace2_init :
-  finite_valid_trace_init_to ParityVLSM
-    parity_trace2_init_first_state parity_trace2_init_last_state parity_trace2_init.
+Example radix_valid_trace2_init :
+  finite_valid_trace_init_to RadixVLSM
+    radix_trace2_init_first_state radix_trace2_init_last_state radix_trace2_init.
 Proof.
-  constructor; [| by unfold parity_trace2_init_first_state; cbn; red; lia].
+  constructor; [| by unfold radix_trace2_init_first_state; cbn; red; lia].
   repeat apply finite_valid_trace_from_to_extend.
   - by eapply finite_valid_trace_from_to_empty, input_valid_transition_destination,
-      parity_valid_transition_2'.
-  - by apply parity_valid_transition_2'.
-  - by apply parity_valid_transition_1'.
+      radix_valid_transition_2'.
+  - by apply radix_valid_transition_2'.
+  - by apply radix_valid_transition_1'.
 Qed.
 
-Example parity_valid_trace2_init_alt :
-  finite_valid_trace_init_to_alt ParityVLSM
-    parity_trace2_init_first_state parity_trace2_init_last_state parity_trace2_init.
+Example radix_valid_trace2_init_alt :
+  finite_valid_trace_init_to_alt RadixVLSM
+    radix_trace2_init_first_state radix_trace2_init_last_state radix_trace2_init.
 Proof.
-  constructor; [| by unfold parity_trace2_init_first_state; cbn; red; lia].
+  constructor; [| by unfold radix_trace2_init_first_state; cbn; red; lia].
   repeat apply mvt_extend; [.. | by apply mvt_empty].
-  - by apply parity_valid_message_prop_mult.
-  - by apply parity_valid_transition_1'.
-  - by cbn; split; unfold parity_trace2_init_first_state; lia.
-  - by apply parity_valid_message_prop_mult.
-  - by apply parity_valid_transition_2'.
-  - by cbn; split; unfold parity_trace2_init_first_state; lia.
+  - by apply radix_valid_message_prop_mult.
+  - by apply radix_valid_transition_1'.
+  - by cbn; split; unfold radix_trace2_init_first_state; lia.
+  - by apply radix_valid_message_prop_mult.
+  - by apply radix_valid_transition_2'.
+  - by cbn; split; unfold radix_trace2_init_first_state; lia.
 Qed.
 
 (**
@@ -353,38 +345,38 @@ Qed.
   without its last transition is constrained.
 *)
 
-Example parity_constrained_trace2_init :
-  finite_constrained_trace_init_to ParityVLSM
-    parity_trace2_init_first_state parity_trace2_init_last_state parity_trace2_init.
+Example radix_constrained_trace2_init :
+  finite_constrained_trace_init_to RadixVLSM
+    radix_trace2_init_first_state radix_trace2_init_last_state radix_trace2_init.
 Proof.
   intros.
   apply VLSM_incl_finite_valid_trace_init_to.
   - by apply vlsm_incl_pre_loaded.
-  - by apply parity_valid_trace2_init; lia.
+  - by apply radix_valid_trace2_init; lia.
 Qed.
 
 (**
-  The trace is valid (in the preloaded Parity VLSM) without
+  The trace is valid (in the preloaded Radix VLSM) without
   its last element and appending it to the end also gives
-  a valid trace (in the preloaded Parity VLSM).
+  a valid trace (in the preloaded Radix VLSM).
   It follows that the full trace is constrained in
-  the original Parity VLSM.
+  the original Radix VLSM.
 *)
 
-Example parity_constrained_trace2 :
-  finite_constrained_trace_init_to ParityVLSM
-    parity_trace2_init_first_state parity_trace2_last_state parity_trace2.
+Example radix_constrained_trace2 :
+  finite_constrained_trace_init_to RadixVLSM
+    radix_trace2_init_first_state radix_trace2_last_state radix_trace2.
 Proof.
-  destruct parity_constrained_trace2_init as [Hfvt Hisp].
+  destruct radix_constrained_trace2_init as [Hfvt Hisp].
   split; [| done].
   eapply (extend_right_finite_trace_from_to _ Hfvt).
   repeat split.
   - by eapply finite_valid_trace_from_to_last_pstate.
   - by apply any_message_is_valid_in_preloaded.
-  - by unfold parity_trace2_init_last_state.
+  - by unfold radix_trace2_init_last_state.
   - by lia.
   - cbn; f_equal.
-    + by unfold parity_trace2_init_last_state; lia.
+    + by unfold radix_trace2_init_last_state; lia.
     + by f_equal; nia.
 Qed.
 
@@ -393,14 +385,14 @@ Qed.
   The last transition of a valid trace is valid.
 *)
 
-Lemma parity_example_valid_transition :
-  input_valid_transition ParityVLSM parity_label
+Lemma radix_example_valid_transition :
+  input_valid_transition RadixVLSM radix_label
     (multiplier, Some multiplier) (0, Some (multiplier ^ 2)).
 Proof.
   repeat split; [| | by lia.. |].
   - apply initial_state_is_valid.
-    by unfold parity_trace2_init_first_state; cbn; red; lia.
-  - by apply parity_valid_message_prop_mult.
+    by unfold radix_trace2_init_first_state; cbn; red; lia.
+  - by apply radix_valid_message_prop_mult.
   - by cbn; do 2 f_equal; lia.
 Qed.
 
@@ -409,49 +401,49 @@ Qed.
   The last transition of a constrained trace is constrained.
 *)
 
-Example parity_example_constrained_transition :
-  input_valid_transition (pre_loaded_with_all_messages_vlsm ParityVLSM) parity_label
+Example radix_example_constrained_transition :
+  input_valid_transition (pre_loaded_with_all_messages_vlsm RadixVLSM) radix_label
     (multiplier + 1, Some (multiplier + 1)) (0, Some (multiplier ^ 2 + multiplier)).
 Proof.
   apply (finite_valid_trace_from_to_last_transition
-    (pre_loaded_with_all_messages_vlsm ParityVLSM)
-    parity_trace2_init_first_state parity_trace2_last_state parity_trace2_init
-    parity_trace2 parity_trace2_last_item); [| done].
-  by apply parity_constrained_trace2.
+    (pre_loaded_with_all_messages_vlsm RadixVLSM)
+    radix_trace2_init_first_state radix_trace2_last_state radix_trace2_init
+    radix_trace2 radix_trace2_last_item); [| done].
+  by apply radix_constrained_trace2.
 Qed.
 
-(** ** Parity VLSM Properties *)
+(** ** Radix VLSM Properties *)
 
 (** *** Inclusion into preloaded with all messages *)
 
-Lemma parity_valid_is_constrained :
-  VLSM_incl ParityVLSM (pre_loaded_with_all_messages_vlsm ParityVLSM).
+Lemma radix_valid_is_constrained :
+  VLSM_incl RadixVLSM (pre_loaded_with_all_messages_vlsm RadixVLSM).
 Proof.
   by apply vlsm_incl_pre_loaded_with_all_messages_vlsm.
 Qed.
 
 (** *** Constrained messages are positive even integers *)
 
-Lemma parity_constrained_messages_left :
+Lemma radix_constrained_messages_left :
   multiplier > 0 ->
-  forall (m : ParityMessage),
-    constrained_message_prop ParityVLSM m ->
+  forall (m : RadixMessage),
+    constrained_message_prop RadixVLSM m ->
     exists (j : Z), m = multiplier * j /\ j > 1.
 Proof.
   intros Hgt0 m ([s []] & [] & s' & (_ & _ & []) & Ht).
   inversion Ht; subst.
-  by exists p; split; lia.
+  by exists r; split; lia.
 Qed.
 
-Lemma parity_constrained_messages_right :
+Lemma radix_constrained_messages_right :
   multiplier > 0 ->
-  forall (m : ParityMessage),
+  forall (m : RadixMessage),
     (exists (j : Z), m = multiplier * j) -> m > multiplier ->
-    constrained_message_prop ParityVLSM m.
+    constrained_message_prop RadixVLSM m.
 Proof.
   intros Hgt0 m (j & Hj) Hmgt0.
   unfold constrained_message_prop_direct, can_emit.
-  exists (j, Some j), parity_label, 0.
+  exists (j, Some j), radix_label, 0.
   repeat split.
   - by apply initial_state_is_valid; cbn; red; nia.
   - by apply any_message_is_valid_in_preloaded.
@@ -460,54 +452,54 @@ Proof.
   - by cbn; do 2 f_equal; lia.
 Qed.
 
-Lemma parity_constrained_messages :
+Lemma radix_constrained_messages :
   multiplier > 0 ->
-  forall (m : ParityMessage),
-    constrained_message_prop ParityVLSM m <-> (exists (j : Z), m = multiplier * j /\ j > 1).
+  forall (m : RadixMessage),
+    constrained_message_prop RadixVLSM m <-> (exists (j : Z), m = multiplier * j /\ j > 1).
 Proof.
   split.
-  - by apply parity_constrained_messages_left.
-  - by intros [? []]; apply parity_constrained_messages_right; [| exists x | nia].
+  - by apply radix_constrained_messages_left.
+  - by intros [? []]; apply radix_constrained_messages_right; [| exists x | nia].
 Qed.
 
 (** *** Constrained states property *)
 
-Lemma parity_constrained_states_right :
-  forall (st : ParityState),
-    constrained_state_prop ParityVLSM st -> st >= 0.
+Lemma radix_constrained_states_right :
+  forall (st : RadixState),
+    constrained_state_prop RadixVLSM st -> st >= 0.
 Proof.
   induction 1 using valid_state_prop_ind.
-  - by cbn in Hs; unfold ParityComponent_initial_state_prop in Hs; lia.
+  - by cbn in Hs; unfold Radix_initial_state_prop in Hs; lia.
   - destruct l, om, Ht as [(Hs & _ & []) Ht].
     by inversion Ht; subst; cbn in *; lia.
 Qed.
 
-Lemma parity_constrained_states_left :
-  forall (st : ParityState),
-    st >= 0 -> constrained_state_prop ParityVLSM st.
+Lemma radix_constrained_states_left :
+  forall (st : RadixState),
+    st >= 0 -> constrained_state_prop RadixVLSM st.
 Proof.
   intros st Hst.
   apply input_valid_transition_destination
-    with (l := parity_label) (s := st + 2) (om := Some 2) (om' := Some (2 * multiplier)).
+    with (l := radix_label) (s := st + 2) (om := Some 2) (om' := Some (2 * multiplier)).
   repeat split; [| | by lia.. | by cbn; do 2 f_equal; lia].
-  - by apply initial_state_is_valid; cbn; unfold ParityComponent_initial_state_prop; lia.
+  - by apply initial_state_is_valid; cbn; unfold Radix_initial_state_prop; lia.
   - by apply any_message_is_valid_in_preloaded.
 Qed.
 
-Lemma parity_constrained_states :
-  forall (st : ParityState),
-    constrained_state_prop ParityVLSM st <-> st >= 0.
+Lemma radix_constrained_states :
+  forall (st : RadixState),
+    constrained_state_prop RadixVLSM st <-> st >= 0.
 Proof.
   split.
-  - by apply parity_constrained_states_right.
-  - by apply parity_constrained_states_left.
+  - by apply radix_constrained_states_right.
+  - by apply radix_constrained_states_left.
 Qed.
 
 (** *** Positive powers of the multiplier are valid messages *)
 
-Lemma parity_valid_messages_powers_of_mult_right :
-  forall (m : ParityMessage),
-    valid_message_prop ParityVLSM m ->
+Lemma radix_valid_messages_powers_of_mult_right :
+  forall (m : RadixMessage),
+    valid_message_prop RadixVLSM m ->
     exists p : Z, p >= 1 /\ m = multiplier ^ p.
 Proof.
   intros m [s Hvsm].
@@ -527,9 +519,9 @@ Proof.
     by rewrite <- Z.pow_succ_r; [| lia].
 Qed.
 
-Lemma parity_valid_messages_powers_of_mult_left :
+Lemma radix_valid_messages_powers_of_mult_left :
   forall (p : Z),
-    p >= 1 -> valid_message_prop ParityVLSM (multiplier ^ p).
+    p >= 1 -> valid_message_prop RadixVLSM (multiplier ^ p).
 Proof.
   intros p Hp.
   assert (Hle : 0 <= p - 1) by lia.
@@ -541,7 +533,7 @@ Proof.
   intros x Hxgt0 Hindh.
   pose (msgin := multiplier ^ (x + 1)).
   apply emitted_messages_are_valid.
-  exists (msgin, Some (multiplier ^ (x + 1))), parity_label, 0.
+  exists (msgin, Some (multiplier ^ (x + 1))), radix_label, 0.
   repeat split.
   - by apply initial_state_is_valid; cbn; red; lia.
   - by apply Hindh.
@@ -551,34 +543,34 @@ Proof.
   - by cbn; rewrite <- Z.pow_succ_r, Z.add_succ_l; [do 2 f_equal; lia | lia].
 Qed.
 
-Lemma parity_valid_messages_powers_of_mult :
-  forall (m : ParityMessage),
-    valid_message_prop ParityVLSM m
+Lemma radix_valid_messages_powers_of_mult :
+  forall (m : RadixMessage),
+    valid_message_prop RadixVLSM m
       <->
     exists p : Z, p >= 1 /\ m = multiplier ^ p.
 Proof.
   split.
-  - by intros; apply parity_valid_messages_powers_of_mult_right.
-  - by intros (p & Hpgt0 & [= ->]); apply parity_valid_messages_powers_of_mult_left.
+  - by intros; apply radix_valid_messages_powers_of_mult_right.
+  - by intros (p & Hpgt0 & [= ->]); apply radix_valid_messages_powers_of_mult_left.
 Qed.
 
 (**
-  The constrained transition from [parity_example_constrained_transition]
+  The constrained transition from [radix_example_constrained_transition]
   is not also valid.
 *)
-Example parity_example_constrained_transition_not_valid :
-  ~ input_valid_transition ParityVLSM parity_label
+Example radix_example_constrained_transition_not_valid :
+  ~ input_valid_transition RadixVLSM radix_label
     (multiplier + 1, Some (multiplier + 1)) (0, Some (multiplier ^ 2 + multiplier)).
 Proof.
   intros [(_ & Hm & _) _].
-  apply parity_valid_messages_powers_of_mult in Hm as (p & Hp & Heq).
+  apply radix_valid_messages_powers_of_mult in Hm as (p & Hp & Heq).
   rewrite <- (Z.succ_pred p) in Heq.
   rewrite Z.pow_succ_r in Heq by lia.
   assert (Hmul : multiplier * (multiplier ^ Z.pred p - 1) = 1) by lia.
   by apply Z.eq_mul_1_nonneg in Hmul as []; lia.
 Qed.
 
-End sec_parity_vlsm.
+End sec_radix_vlsm.
 
 Section sec_composition.
 
@@ -589,33 +581,33 @@ Context
   `{FinSet index indexSet}
   .
 
-Definition indexed_parity_vlsms (i : index) : VLSM ParityMessage :=
-  ParityVLSM (multipliers i).
+Definition indexed_radix_vlsms (i : index) : VLSM RadixMessage :=
+  RadixVLSM (multipliers i).
 
 Context
-  (parity_constraint : composite_label indexed_parity_vlsms ->
-    composite_state indexed_parity_vlsms * option ParityMessage -> Prop)
+  (radix_constraint : composite_label indexed_radix_vlsms ->
+    composite_state indexed_radix_vlsms * option RadixMessage -> Prop)
   .
 
-Definition parity_composite_vlsm : VLSM ParityMessage :=
-  composite_vlsm indexed_parity_vlsms parity_constraint.
+Definition radix_composite_vlsm : VLSM RadixMessage :=
+  composite_vlsm indexed_radix_vlsms radix_constraint.
 
 Lemma composite_state_pos
-  (s : composite_state indexed_parity_vlsms)
-  (Hs : valid_state_prop parity_composite_vlsm s) :
+  (s : composite_state indexed_radix_vlsms)
+  (Hs : valid_state_prop radix_composite_vlsm s) :
     forall (i : index), s i >= 0.
 Proof.
   intros i.
-  apply parity_constrained_states_right with (multipliers i).
-  by apply (valid_state_project_preloaded ParityMessage indexed_parity_vlsms parity_constraint).
+  apply radix_constrained_states_right with (multipliers i).
+  by apply (valid_state_project_preloaded RadixMessage indexed_radix_vlsms radix_constraint).
 Qed.
 
 (**
   Any valid message can be expressed as a non-empty product of powers
   of the multipliers associated to the components.
 *)
-Lemma composition_valid_messages_powers_of_mults_right (m : ParityMessage) :
-  valid_message_prop parity_composite_vlsm m ->
+Lemma composition_valid_messages_powers_of_mults_right (m : RadixMessage) :
+  valid_message_prop radix_composite_vlsm m ->
   exists (f : fsfun index 0%nat),
     fin_supp f <> [] /\ m = fsfun_prod multipliers f.
 Proof.
@@ -629,7 +621,7 @@ Proof.
     by rewrite <- Hmi, mi, prod_powers_delta.
   - destruct l as (k & lk).
     destruct om; [| done].
-    destruct (IHHvsm2 p) as (f & Hdomf & ->); [done |].
+    destruct (IHHvsm2 r) as (f & Hdomf & ->); [done |].
     inversion Ht.
     exists (succ_fsfun f k).
     split; [| by rewrite fsfun_prod_succ].
@@ -647,15 +639,15 @@ Context
   `{Inhabited index}
   .
 
-Definition free_parity_composite_vlsm : VLSM ParityMessage :=
-  free_composite_vlsm (indexed_parity_vlsms multipliers).
+Definition free_radix_composite_vlsm : VLSM RadixMessage :=
+  free_composite_vlsm (indexed_radix_vlsms multipliers).
 
-#[local] Lemma free_parity_composite_vlsm_emits_multiplier :
-  forall (m : ParityMessage),
-    valid_message_prop free_parity_composite_vlsm m ->
+#[local] Lemma free_radix_composite_vlsm_emits_multiplier :
+  forall (m : RadixMessage),
+    valid_message_prop free_radix_composite_vlsm m ->
     m >= 2 ->
   forall (n : index),
-  input_valid_transition free_parity_composite_vlsm (existT n parity_label)
+  input_valid_transition free_radix_composite_vlsm (existT n radix_label)
 (update (const 1) n (m + 1), Some m)
 (const 1, Some (multipliers n * m)).
 Proof.
@@ -674,15 +666,15 @@ Proof.
 Qed.
 
 Lemma composition_valid_messages_powers_of_mults_left
-  (Hmpos : forall (i : index), multipliers i > 1) (m : ParityMessage)
+  (Hmpos : forall (i : index), multipliers i > 1) (m : RadixMessage)
   (f : fsfun index 0%nat) :
     fin_supp f <> [] /\ m = fsfun_prod multipliers f ->
-    valid_message_prop free_parity_composite_vlsm m.
+    valid_message_prop free_radix_composite_vlsm m.
 Proof.
   intros [Hpowgeq1 Hm]; revert f Hpowgeq1 m Hm.
   apply (nat_fsfun_ind (fun (f : fsfun index 0%nat) => fin_supp f <> [] ->
-    forall m : ParityMessage, m = fsfun_prod multipliers f ->
-    valid_message_prop free_parity_composite_vlsm m)); [| done |].
+    forall m : RadixMessage, m = fsfun_prod multipliers f ->
+    valid_message_prop free_radix_composite_vlsm m)); [| done |].
   - intros f1 f2 Heq Hall Hi m Hm.
     eapply Hall; [| by rewrite Heq].
     contradict Hi.
@@ -693,7 +685,7 @@ Proof.
     + rewrite fsfun_prod_succ, Heq, fsfun_prod_zero in Hm.
       apply initial_message_is_valid. exists n.
       by unshelve eexists (exist _ m _); cbn; lia.
-    + assert (Hmvalid : valid_message_prop free_parity_composite_vlsm (fsfun_prod multipliers f0)).
+    + assert (Hmvalid : valid_message_prop free_radix_composite_vlsm (fsfun_prod multipliers f0)).
       {
         apply IHf0; [| done].
         assert (Hinh : fin_supp (succ_fsfun f0' n') <> []).
@@ -716,12 +708,12 @@ Proof.
       }
       specialize (Hmpos n').
       by eapply input_valid_transition_out,
-        free_parity_composite_vlsm_emits_multiplier; [| lia].
+        free_radix_composite_vlsm_emits_multiplier; [| lia].
 Qed.
 
 Lemma composition_valid_messages_powers_of_mults
-  (Hmpos : forall (i : index), multipliers i > 1) (m : ParityMessage) :
-    valid_message_prop free_parity_composite_vlsm m <->
+  (Hmpos : forall (i : index), multipliers i > 1) (m : RadixMessage) :
+    valid_message_prop free_radix_composite_vlsm m <->
   exists (f : fsfun index 0%nat),
     fin_supp f <> [] /\ m = fsfun_prod multipliers f.
 Proof.
@@ -735,8 +727,8 @@ Proof.
 Qed.
 
 Lemma composition_valid_message_ge_2
-  (Hmpos : forall (i : index), multipliers i > 1) (m : ParityMessage) :
-  valid_message_prop free_parity_composite_vlsm m -> m >= 2.
+  (Hmpos : forall (i : index), multipliers i > 1) (m : RadixMessage) :
+  valid_message_prop free_radix_composite_vlsm m -> m >= 2.
 Proof.
   intro Hv.
   apply composition_valid_messages_powers_of_mults in Hv
@@ -747,7 +739,7 @@ Qed.
 
 End sec_free_composition.
 
-Section sec_parity23.
+Section sec_radix23.
 
 Inductive index23 := two | three.
 
@@ -769,25 +761,25 @@ Proof.
   - by intros []; set_solver.
 Qed.
 
-Definition parity_constraint
-  (l : composite_label (indexed_parity_vlsms multipliers23))
-  (sm : composite_state (indexed_parity_vlsms multipliers23) * option ParityMessage) : Prop :=
+Definition radix_constraint
+  (l : composite_label (indexed_radix_vlsms multipliers23))
+  (sm : composite_state (indexed_radix_vlsms multipliers23) * option RadixMessage) : Prop :=
     let i := projT1 l in
-    let (s', _) := composite_transition (indexed_parity_vlsms multipliers23) l sm in
+    let (s', _) := composite_transition (indexed_radix_vlsms multipliers23) l sm in
     Z.Even (((fst sm) i) + (s' i)).
 
-Definition parity_composite_vlsm23 :=
-  parity_composite_vlsm multipliers23 parity_constraint.
+Definition radix_composite_vlsm23 :=
+  radix_composite_vlsm multipliers23 radix_constraint.
 
-Definition final_state (s : composite_state (indexed_parity_vlsms multipliers23)) :=
-  valid_state_prop parity_composite_vlsm23 s /\
+Definition final_state (s : composite_state (indexed_radix_vlsms multipliers23)) :=
+  valid_state_prop radix_composite_vlsm23 s /\
   ~ exists
-    (l : composite_label (indexed_parity_vlsms multipliers23))
-    (om : option ParityMessage)
-    (som' : composite_state (indexed_parity_vlsms multipliers23) * option ParityMessage),
-      input_valid_transition parity_composite_vlsm23 l (s, om) som'.
+    (l : composite_label (indexed_radix_vlsms multipliers23))
+    (om : option RadixMessage)
+    (som' : composite_state (indexed_radix_vlsms multipliers23) * option RadixMessage),
+      input_valid_transition radix_composite_vlsm23 l (s, om) som'.
 
-Definition statenm (n m : Z) : composite_state (indexed_parity_vlsms multipliers23) :=
+Definition statenm (n m : Z) : composite_state (indexed_radix_vlsms multipliers23) :=
   fun (i : index23) => match i with two => n | three => m end.
 
 Definition state00 := statenm 0 0.
@@ -807,26 +799,26 @@ Definition state22 := statenm 2 2.
 Definition state02 := statenm 0 2.
 
 Example valid_statenm_geq1 (n m : Z) (Hn : n >= 1) (Hm : m >= 1) :
-  valid_state_prop parity_composite_vlsm23 (statenm n m).
+  valid_state_prop radix_composite_vlsm23 (statenm n m).
 Proof.
   by apply initial_state_is_valid; intros []; cbn; red.
 Qed.
 
-Example valid_state11 : valid_state_prop parity_composite_vlsm23 state11.
+Example valid_state11 : valid_state_prop radix_composite_vlsm23 state11.
 Proof. by apply (valid_statenm_geq1 1 1); lia. Qed.
 
-Example valid_state00 : valid_state_prop parity_composite_vlsm23 state00.
+Example valid_state00 : valid_state_prop radix_composite_vlsm23 state00.
 Proof.
   apply input_valid_transition_destination
-    with (l := existT three parity_label) (s := state02) (om := Some 2) (om' := Some 6).
+    with (l := existT three radix_label) (s := state02) (om := Some 2) (om' := Some 6).
   repeat split.
   - apply input_valid_transition_destination
-      with (l := existT two parity_label) (s := state22) (om := Some 2) (om' := Some 4).
+      with (l := existT two radix_label) (s := state22) (om := Some 2) (om' := Some 4).
     repeat split.
     + by apply valid_statenm_geq1.
     + apply initial_message_is_valid.
       exists two.
-      assert (Hinit : initial_message_prop (indexed_parity_vlsms multipliers23 two) 2) by done.
+      assert (Hinit : initial_message_prop (indexed_radix_vlsms multipliers23 two) 2) by done.
       by exists (exist _ 2 Hinit).
     + by cbn; lia.
     + by lia.
@@ -834,7 +826,7 @@ Proof.
     + by cbn; f_equal; extensionality i; destruct i; cbn; state_update_simpl; cbn; lia.
   - apply initial_message_is_valid.
     exists two.
-    assert (Hinit : initial_message_prop (indexed_parity_vlsms multipliers23 two) 2) by done.
+    assert (Hinit : initial_message_prop (indexed_radix_vlsms multipliers23 two) 2) by done.
     by exists (exist _ 2 Hinit).
   - by unfold state02; cbn; lia.
   - by lia.
@@ -842,15 +834,15 @@ Proof.
   - by cbn; f_equal; extensionality i; destruct i; cbn; state_update_simpl; cbn; lia.
 Qed.
 
-Example valid_state01 : valid_state_prop parity_composite_vlsm23 state01.
+Example valid_state01 : valid_state_prop radix_composite_vlsm23 state01.
 Proof.
   apply input_valid_transition_destination
-    with (l := existT two parity_label) (s := state21) (om := Some 2) (om' := Some 4).
+    with (l := existT two radix_label) (s := state21) (om := Some 2) (om' := Some 4).
   repeat split.
   - by apply valid_statenm_geq1.
   - apply initial_message_is_valid.
     exists two.
-    assert (Hinit : initial_message_prop (indexed_parity_vlsms multipliers23 two) 2) by done.
+    assert (Hinit : initial_message_prop (indexed_radix_vlsms multipliers23 two) 2) by done.
     by exists (exist _ 2 Hinit).
   - by cbn; lia.
   - by lia.
@@ -858,15 +850,15 @@ Proof.
   - by cbn; f_equal; extensionality i; destruct i; cbn; state_update_simpl; cbn; lia.
 Qed.
 
-Example valid_state10 : valid_state_prop parity_composite_vlsm23 state10.
+Example valid_state10 : valid_state_prop radix_composite_vlsm23 state10.
 Proof.
   apply input_valid_transition_destination
-    with (l := existT three parity_label) (s := state12) (om := Some 2) (om' := Some 6).
+    with (l := existT three radix_label) (s := state12) (om := Some 2) (om' := Some 6).
   repeat split.
   - by apply valid_statenm_geq1.
   - apply initial_message_is_valid.
     exists two.
-    assert (Hinit : initial_message_prop (indexed_parity_vlsms multipliers23 two) 2) by done.
+    assert (Hinit : initial_message_prop (indexed_radix_vlsms multipliers23 two) 2) by done.
     by exists (exist _ 2 Hinit).
   - by cbn; lia.
   - by lia.
@@ -874,7 +866,7 @@ Proof.
   - by cbn; f_equal; extensionality i; destruct i; cbn; state_update_simpl; cbn; lia.
 Qed.
 
-Lemma final_state_prop23_left (s : composite_state (indexed_parity_vlsms multipliers23)) :
+Lemma final_state_prop23_left (s : composite_state (indexed_radix_vlsms multipliers23)) :
   (s = state00 \/ s = state01 \/ s = state10 \/ s = state11) -> final_state s.
 Proof.
   intros Hcases.
@@ -885,16 +877,16 @@ Proof.
     + by apply valid_state10.
     + by apply valid_state11.
   - intros ([i li] & om & som' & (Hs & Hom & Hv & Hc) & Ht).
-    unfold parity_constraint in Hc.
+    unfold radix_constraint in Hc.
     replace (composite_transition _ _ _) with som' in Hc.
     destruct om; [| done].
     cbn in *; subst.
     state_update_simpl.
-    assert (Z.Even p) as [n Hp] by (destruct Hc as [n Hc]; exists (s i - n); lia).
+    assert (Z.Even r) as [n Hp] by (destruct Hc as [n Hc]; exists (s i - n); lia).
     by destruct Hcases as [Hst |[Hst |[Hst | Hst]]]; subst; destruct i; cbn in *; lia.
 Qed.
 
-Lemma final_state_prop23_right (s : composite_state (indexed_parity_vlsms multipliers23)) :
+Lemma final_state_prop23_right (s : composite_state (indexed_radix_vlsms multipliers23)) :
   final_state s ->
     (s two = 0 /\ s three = 0) \/ (s two = 0 /\ s three = 1) \/
     (s two = 1 /\ s three = 0) \/ (s two = 1 /\ s three = 1).
@@ -912,24 +904,24 @@ Proof.
   }
   contradict Hfinal.
   clear n.
-  exists (existT i parity_label), (Some 2),
-    (state_update (indexed_parity_vlsms multipliers23) s i (s i - 2), Some (multipliers23 i * 2)).
+  exists (existT i radix_label), (Some 2),
+    (state_update (indexed_radix_vlsms multipliers23) s i (s i - 2), Some (multipliers23 i * 2)).
   repeat split; [done | ..].
   - apply initial_message_is_valid.
     exists two.
-    assert (Hinit : initial_message_prop (indexed_parity_vlsms multipliers23 two) 2) by done.
+    assert (Hinit : initial_message_prop (indexed_radix_vlsms multipliers23 two) 2) by done.
     by exists (exist _ 2 Hinit).
   - by lia.
   - by lia.
   - by cbn; state_update_simpl; exists (s i - 1); lia.
 Qed.
 
-End sec_parity23.
+End sec_radix23.
 
 (** ** A VLSM composition for all primes
 
   In the following section we give an example of a composition with an infinite
-  number of [ParityVLSM] components, one for each prime number.
+  number of [RadixVLSM] components, one for each prime number.
 
   Then we characterize the valid messages for this composition to be precisely
   all natural numbers larger than 1.
@@ -940,7 +932,7 @@ End sec_parity23.
 Section sec_primes_vlsm_composition.
 
 Definition primes_vlsm_composition : VLSM Z :=
-  free_parity_composite_vlsm (fun p : primes => `p).
+  free_radix_composite_vlsm (fun p : primes => `p).
 
 Lemma primes_vlsm_composition_valid_message_char :
   forall (m : Z),
@@ -969,11 +961,11 @@ Qed.
 Theorem component_projection_validator_prop_primes :
   forall (p : primes),
     component_projection_validator_prop
-      (indexed_parity_vlsms (fun p : primes => ` p))
+      (indexed_radix_vlsms (fun p : primes => ` p))
       (fun _ _ => True) p.
 Proof.
   intros p lp sp [m|] (Hsp & _ & []).
-  exists (lift_to_composite_state' (indexed_parity_vlsms (fun p : primes => `p)) p sp).
+  exists (lift_to_composite_state' (indexed_radix_vlsms (fun p : primes => `p)) p sp).
   repeat split; [by state_update_simpl | | | by state_update_simpl | done].
   - apply initial_state_is_valid.
     intros p'; cbn; red.
@@ -997,12 +989,12 @@ Definition even_constrained_primes_composition : VLSM Z :=
   constrained_vlsm primes_vlsm_composition EvenConstraint.
 
 #[local] Lemma even_constrained_primes_composition_emits_multiplier :
-  forall (m : ParityMessage),
+  forall (m : RadixMessage),
     valid_message_prop even_constrained_primes_composition m ->
     m >= 2 ->
     Z.Even m ->
   forall (n : primes),
-  input_valid_transition even_constrained_primes_composition (existT n parity_label)
+  input_valid_transition even_constrained_primes_composition (existT n radix_label)
   (update (const 1) n (m + 1), Some m)
   (const 1, Some (` n * m)).
 Proof.
@@ -1025,7 +1017,7 @@ Lemma even_constrained_primes_composition_valid_messages_left (m : Z) :
   m > 1 -> Z.Even m -> valid_message_prop even_constrained_primes_composition m.
 Proof.
   intros Hm1 Hmeven.
-  assert (Hinit : composite_initial_message_prop (indexed_parity_vlsms (fun p : primes => `p)) 2)
+  assert (Hinit : composite_initial_message_prop (indexed_radix_vlsms (fun p : primes => `p)) 2)
     by (unshelve eexists (dexist 2 prime_2), (exist _ 2 _); done).
   destruct (decide (m = 2)) as [-> | Hm2]; [by apply initial_message_is_valid |].
   destruct Hmeven as [n ->].
@@ -1083,13 +1075,13 @@ Qed.
 Lemma even_constrained_primes_composition_no_validator :
   forall (p : primes),
     ~ component_projection_validator_prop
-        (indexed_parity_vlsms (fun p : primes => ` p))
+        (indexed_radix_vlsms (fun p : primes => ` p))
         EvenConstraint p.
 Proof.
   intros p Hnv.
   cut (input_valid
     (pre_loaded_with_all_messages_vlsm
-      (indexed_parity_vlsms (λ p0 : primes, `p0) p)) () (3, Some 3)).
+      (indexed_radix_vlsms (λ p0 : primes, `p0) p)) () (3, Some 3)).
   {
     intro Hiv.
     apply Hnv in Hiv as (s & _ & _ & _ & _ & Hc).
@@ -1105,12 +1097,12 @@ Qed.
   equivalent to the global constraint we can recover validation.
 *)
 Inductive LocalEvenConstraint (mult : Z) :
-  label (ParityVLSM mult) -> state (ParityVLSM mult) * option Z -> Prop :=
+  label (RadixVLSM mult) -> state (RadixVLSM mult) * option Z -> Prop :=
 | local_even_constraint : forall l s m, Z.Even m ->
     LocalEvenConstraint mult l (s, Some m).
 
-Definition even_prime_vlsms (p : primes) : VLSM ParityMessage :=
-  constrained_vlsm (ParityVLSM (`p)) (LocalEvenConstraint (`p)).
+Definition even_prime_vlsms (p : primes) : VLSM RadixMessage :=
+  constrained_vlsm (RadixVLSM (`p)) (LocalEvenConstraint (`p)).
 
 (**
   Adding the local constraint to each component does not change the behavior
@@ -1137,7 +1129,7 @@ Lemma even_constrained_primes_composition_all_validators :
 Proof.
   intros p lp sp [m |] (Hsp & _ & [[] Hc]).
   inversion Hc as [? ? ? Heven]; subst.
-  exists (lift_to_composite_state' (indexed_parity_vlsms (fun p : primes => `p)) p sp).
+  exists (lift_to_composite_state' (indexed_radix_vlsms (fun p : primes => `p)) p sp).
   repeat split; [by state_update_simpl | | | by state_update_simpl | done..].
   - apply initial_state_is_valid.
     intro p'; cbn; red.
