theories/VLSM/Core/VLSM.v
@@ -2788,3 +2788,13 @@ Proof.
 Qed.
 
 End sec_finite_valid_trace_init_to_alt.
+
+(** Custom tactic used to simplify proofs of valid VLSM transitions. *)
+Ltac app_valid_tran :=
+  repeat split; cbn; try done;
+  match goal with
+  | |- option_valid_message_prop _ _ => by apply initial_message_is_valid
+  | |- option_valid_message_prop _ _ => eapply emitted_messages_are_valid
+  | |- valid_state_prop _ _ => by apply initial_state_is_valid
+  | |- valid_state_prop _ _ => eapply input_valid_transition_destination
+  end.
